src/impl/TLS13.Impl.Driver.Pairing.fsti
@@ -362,7 +362,7 @@ let client_server_driver_supported_profile_application_record_state_inputs
     server.CS.cs_model
 
 noextract
-let client_server_driver_supported_profile_projected_state_inputs
+let client_server_driver_remaining_semantic_projection_inputs
   (client:CS.connection_state)
   (server:CS.connection_state)
   : prop =
@@ -370,6 +370,13 @@ let client_server_driver_supported_profile_projected_state_inputs
   client_server_driver_supported_profile_application_record_state_inputs
     client
     server
+
+noextract
+let client_server_driver_supported_profile_projected_state_inputs
+  (client:CS.connection_state)
+  (server:CS.connection_state)
+  : prop =
+  client_server_driver_remaining_semantic_projection_inputs client server
 
 noextract
 let client_server_driver_supported_profile_state_inputs
@@ -432,7 +439,7 @@ let client_server_driver_key_material_no_read_ahead_component_inputs
   client_server_driver_supported_profile_state_inputs client server
 
 noextract
-let client_server_driver_key_material_no_read_ahead_projection_inputs
+let client_server_driver_public_success_transport_inputs
   (client:CS.connection_state)
   (server:CS.connection_state)
   (client_received:B.bytes)
@@ -452,8 +459,25 @@ let client_server_driver_key_material_no_read_ahead_projection_inputs
     client_received
     client_sent
     server_received
+    server_sent
+
+noextract
+let client_server_driver_key_material_no_read_ahead_projection_inputs
+  (client:CS.connection_state)
+  (server:CS.connection_state)
+  (client_received:B.bytes)
+  (client_sent:B.bytes)
+  (server_received:B.bytes)
+  (server_sent:B.bytes)
+  : prop =
+  client_server_driver_public_success_transport_inputs
+    client
+    server
+    client_received
+    client_sent
+    server_received
     server_sent /\
-  client_server_driver_supported_profile_projected_state_inputs client server
+  client_server_driver_remaining_semantic_projection_inputs client server
 
 val lemma_client_server_driver_key_material_agrees_from_no_read_ahead
   (client:CS.connection_state)
@@ -559,6 +583,41 @@ val lemma_client_server_driver_key_material_agrees_from_public_success_projectio
           client_sent
           server_received
           server_sent)
+      (ensures
+        client_server_driver_supported_profile_derived_state_inputs
+          client
+          server /\
+        CS.supported_profile_all_derived_key_material_agrees client server /\
+        CS.supported_profile_client_server_key_material_inputs_agree
+          client
+          server /\
+        paired_driver_transport_logs_exact
+          client
+          server
+          client_received
+          client_sent
+          server_received
+          server_sent /\
+        CS.paired_wire_logs client server /\
+        CS.supported_profile_client_server_key_material_agrees client server)
+
+val lemma_client_server_driver_key_material_agrees_from_public_success_transport_and_semantics
+  (client:CS.connection_state)
+  (server:CS.connection_state)
+  (client_received:B.bytes)
+  (client_sent:B.bytes)
+  (server_received:B.bytes)
+  (server_sent:B.bytes)
+  : Lemma
+      (requires
+        client_server_driver_public_success_transport_inputs
+          client
+          server
+          client_received
+          client_sent
+          server_received
+          server_sent /\
+        client_server_driver_remaining_semantic_projection_inputs client server)
       (ensures
         client_server_driver_supported_profile_derived_state_inputs
           client
